move-sui: add test that is supposed to panic

CoqOfRust/move_sui/simulations/move_binary_format/errors.v
@@ -32,7 +32,8 @@ Module Location.
   .
 End Location.
 
-Module VMError_.
+(** We merge [VMError] and [VMError_]. *)
+Module VMError.
   Record t : Set := {
     major_status  : StatusCode.t;
     sub_status    : option Z;
@@ -42,13 +43,10 @@ Module VMError_.
     indices       : list (IndexKind.t * TableIndex.t);
     offsets       : list (FunctionDefinitionIndex.t * CodeOffset.t);
   }.
-End VMError_.
-
-Module VMError.
-  Definition t := VMError_.t.
 End VMError.
 
-Module PartialVMError_.
+(** We merge [PartialVMError] and [PartialVMError_]. *)
+Module PartialVMError.
   Record t : Set := {
     major_status  : StatusCode.t;
     sub_status    : option Z;
@@ -57,190 +55,172 @@ Module PartialVMError_.
     indices       : list (IndexKind.t * TableIndex.t);
     offsets       : list (FunctionDefinitionIndex.t * CodeOffset.t);
   }.
-End PartialVMError_.
 
-(* NOTE: WARNING: 
-  Several impl functions involves `mut Self`. Since they mostly only involves
-  changing the value of a constructed object, I'm being lazy here for now: I 
-  only return the updated value rather than modifying the original value. *)
-Module PartialVMError.
-  Record t : Set := {
-    error : PartialVMError_.t;
-  }.
+  (* 
+  impl PartialVMError {
+      pub fn finish(self, location: Location) -> VMError {
+          let PartialVMError_ {
+              major_status,
+              sub_status,
+              message,
+              exec_state,
+              indices,
+              offsets,
+          } = *self.0;
+          VMError(Box::new(VMError_ {
+              major_status,
+              sub_status,
+              message,
+              exec_state,
+              location,
+              indices,
+              offsets,
+          }))
+      }
 
-  Module Impl_PartialVMError.
-    Definition Self := move_sui.simulations.move_binary_format.errors.PartialVMError.t.
-    (* 
-    impl PartialVMError {
-        pub fn finish(self, location: Location) -> VMError {
-            let PartialVMError_ {
-                major_status,
-                sub_status,
-                message,
-                exec_state,
-                indices,
-                offsets,
-            } = *self.0;
-            VMError(Box::new(VMError_ {
-                major_status,
-                sub_status,
-                message,
-                exec_state,
-                location,
-                indices,
-                offsets,
-            }))
-        }
+      pub fn major_status(&self) -> StatusCode {
+          self.0.major_status
+      }
 
-        pub fn major_status(&self) -> StatusCode {
-            self.0.major_status
-        }
+      pub fn with_sub_status(mut self, sub_status: u64) -> Self {
+          debug_assert!(self.0.sub_status.is_none());
+          self.0.sub_status = Some(sub_status);
+          self
+      }
 
-        pub fn with_sub_status(mut self, sub_status: u64) -> Self {
-            debug_assert!(self.0.sub_status.is_none());
-            self.0.sub_status = Some(sub_status);
-            self
-        }
+      pub fn with_message(mut self, message: String) -> Self {
+          debug_assert!(self.0.message.is_none());
+          self.0.message = Some(message);
+          self
+      }
 
-        pub fn with_message(mut self, message: String) -> Self {
-            debug_assert!(self.0.message.is_none());
-            self.0.message = Some(message);
-            self
-        }
+      pub fn with_exec_state(mut self, exec_state: ExecutionState) -> Self {
+          debug_assert!(self.0.exec_state.is_none());
+          self.0.exec_state = Some(exec_state);
+          self
+      }
 
-        pub fn with_exec_state(mut self, exec_state: ExecutionState) -> Self {
-            debug_assert!(self.0.exec_state.is_none());
-            self.0.exec_state = Some(exec_state);
-            self
-        }
+      pub fn at_index(mut self, kind: IndexKind, index: TableIndex) -> Self {
+          self.0.indices.push((kind, index));
+          self
+      }
 
-        pub fn at_index(mut self, kind: IndexKind, index: TableIndex) -> Self {
-            self.0.indices.push((kind, index));
-            self
-        }
+      pub fn at_indices(mut self, additional_indices: Vec<(IndexKind, TableIndex)>) -> Self {
+          self.0.indices.extend(additional_indices);
+          self
+      }
 
-        pub fn at_indices(mut self, additional_indices: Vec<(IndexKind, TableIndex)>) -> Self {
-            self.0.indices.extend(additional_indices);
-            self
-        }
+      pub fn at_code_offsets(
+          mut self,
+          additional_offsets: Vec<(FunctionDefinitionIndex, CodeOffset)>,
+      ) -> Self {
+          self.0.offsets.extend(additional_offsets);
+          self
+      }
 
-        pub fn at_code_offsets(
-            mut self,
-            additional_offsets: Vec<(FunctionDefinitionIndex, CodeOffset)>,
-        ) -> Self {
-            self.0.offsets.extend(additional_offsets);
-            self
-        }
+      /// Append the message `message` to the message field of the VM status, and insert a seperator
+      /// if the original message is non-empty.
+      pub fn append_message_with_separator(
+          mut self,
+          separator: char,
+          additional_message: String,
+      ) -> Self {
+          match self.0.message.as_mut() {
+              Some(msg) => {
+                  if !msg.is_empty() {
+                      msg.push(separator);
+                  }
+                  msg.push_str(&additional_message);
+              }
+              None => self.0.message = Some(additional_message),
+          };
+          self
+      }
+  }
+  *)
 
-        /// Append the message `message` to the message field of the VM status, and insert a seperator
-        /// if the original message is non-empty.
-        pub fn append_message_with_separator(
-            mut self,
-            separator: char,
-            additional_message: String,
-        ) -> Self {
-            match self.0.message.as_mut() {
-                Some(msg) => {
-                    if !msg.is_empty() {
-                        msg.push(separator);
-                    }
-                    msg.push_str(&additional_message);
-                }
-                None => self.0.message = Some(additional_message),
-            };
-            self
-        }
-    }
-    *)
+  (* 
+  pub fn all_data(
+      self,
+  ) -> (
+      StatusCode,
+      Option<u64>,
+      Option<String>,
+      Option<ExecutionState>,
+      Vec<(IndexKind, TableIndex)>,
+      Vec<(FunctionDefinitionIndex, CodeOffset)>,
+  ) {
+      let PartialVMError_ {
+          major_status,
+          sub_status,
+          message,
+          exec_state,
+          indices,
+          offsets,
+      } = *self.0;
+      (
+          major_status,
+          sub_status,
+          message,
+          exec_state,
+          indices,
+          offsets,
+      )
+  }
+  *)
+  Definition all_data (self : t) :
+      StatusCode.t *
+      option Z *
+      option string *
+      option ExecutionState.t *
+      list (IndexKind.t * TableIndex.t) *
+      list (FunctionDefinitionIndex.t * CodeOffset.t) :=
+  (
+    self.(major_status),
+    self.(sub_status),
+    self.(message),
+    self.(exec_state),
+    self.(indices),
+    self.(offsets)
+  ).
 
-    (* 
-    pub fn all_data(
-        self,
-    ) -> (
-        StatusCode,
-        Option<u64>,
-        Option<String>,
-        Option<ExecutionState>,
-        Vec<(IndexKind, TableIndex)>,
-        Vec<(FunctionDefinitionIndex, CodeOffset)>,
-    ) {
-        let PartialVMError_ {
-            major_status,
-            sub_status,
-            message,
-            exec_state,
-            indices,
-            offsets,
-        } = *self.0;
-        (
-            major_status,
-            sub_status,
-            message,
-            exec_state,
-            indices,
-            offsets,
-        )
-    }
-    *)
-    
-    Definition all_data (self : Self) :
-      (StatusCode.t * (option Z) * (option string) * (option ExecutionState.t) 
-        * (list (IndexKind.t * TableIndex.t)) * (list (FunctionDefinitionIndex.t * CodeOffset.t))) :=
-      let '(PartialVMError.Build_t pvme_) := self in
-        (
-        pvme_.(PartialVMError_.major_status),
-        pvme_.(PartialVMError_.sub_status),
-        pvme_.(PartialVMError_.message),
-        pvme_.(PartialVMError_.exec_state),
-        pvme_.(PartialVMError_.indices),
-        pvme_.(PartialVMError_.offsets)
-        ).
+  (* 
+  pub fn new(major_status: StatusCode) -> Self {
+      Self(Box::new(PartialVMError_ {
+          major_status,
+          sub_status: None,
+          message: None,
+          exec_state: None,
+          indices: vec![],
+          offsets: vec![],
+      }))
+  }
+  *)
+  Definition new (major_status : StatusCode.t) : t :=
+    {|
+      major_status  := major_status;
+      sub_status    := None;
+      message       := None;
+      exec_state    := None;
+      indices       := [];
+      offsets       := [];
+    |}.
 
-    (* 
-    pub fn new(major_status: StatusCode) -> Self {
-        Self(Box::new(PartialVMError_ {
-            major_status,
-            sub_status: None,
-            message: None,
-            exec_state: None,
-            indices: vec![],
-            offsets: vec![],
-        }))
-    }
-    *)
-    Definition new (major_status : StatusCode.t) : Self :=
-      let pvme_ : PartialVMError_.t := {|
-        PartialVMError_.major_status  := major_status;
-        PartialVMError_.sub_status    := None;
-        PartialVMError_.message       := None;
-        PartialVMError_.exec_state    := None;
-        PartialVMError_.indices       := [];
-        PartialVMError_.offsets       := [];
-      |} in
-      PartialVMError.Build_t pvme_.
-
-    (* 
-    pub fn at_code_offset(mut self, function: FunctionDefinitionIndex, offset: CodeOffset) -> Self {
-        self.0.offsets.push((function, offset));
-        self
-    }
-    *)
-    Definition at_code_offset (self : Self) (function : FunctionDefinitionIndex.t) 
-      (offset : CodeOffset.t) : Self :=
-      let '(PartialVMError.Build_t pvme_) := self in
-      let offsets := pvme_.(PartialVMError_.offsets) in
-      let offsets := (function, offset) :: offsets in
-      let pvme_ := pvme_ <| PartialVMError_.offsets := offsets |> in
-      PartialVMError.Build_t pvme_.
-
-  End Impl_PartialVMError.
+  (*
+  pub fn at_code_offset(mut self, function: FunctionDefinitionIndex, offset: CodeOffset) -> Self {
+      self.0.offsets.push((function, offset));
+      self
+  }
+  *)
+  Definition at_code_offset
+      (self : t)
+      (function : FunctionDefinitionIndex.t) 
+      (offset : CodeOffset.t) :
+      t :=
+    self <| offsets := (function, offset) :: self.(offsets) |>.
 End PartialVMError.
 
 (* pub type PartialVMResult<T> = ::std::result::Result<T, PartialVMError>; *)
 Module PartialVMResult.
   Definition t (T : Set) := Result.t T PartialVMError.t.
-
-  Module Impl_PartialVMResult.
-    Definition Self := move_sui.simulations.move_binary_format.errors.PartialVMResult.t.
-  End Impl_PartialVMResult.
 End PartialVMResult.
