CoqOfRust/move_sui/simulations/move_bytecode_verifier/type_safety_tests/mod.v
@@ -117,14 +117,90 @@ fn test_br_true_false_correct_type() {
     }
 }
 *)
-Definition test_br_true_false_correct_type_BrTrue : M!? errors.PartialVMError.t unit :=
-  let code := [file_format.Bytecode.LdTrue; file_format.Bytecode.BrTrue 0] in
+Definition test_br_true_false_correct_type (instr : file_format.Bytecode.t) :
+    M!? errors.PartialVMError.t unit :=
+  let code := [file_format.Bytecode.LdTrue; instr] in
   let module := make_module code in
   let! fun_context := get_fun_context module in
   type_safety.verify module fun_context.
 
-Goal test_br_true_false_correct_type_BrTrue = return!? tt.
+Goal List.Forall
+  (fun instr => test_br_true_false_correct_type instr = return!? tt)
+  [
+    file_format.Bytecode.BrTrue 0;
+    file_format.Bytecode.BrFalse 0
+  ].
 Proof.
-  vm_compute.
-  reflexivity.
+  repeat constructor.
+Qed.
+
+(*
+#[test]
+fn test_br_true_false_wrong_type() {
+    for instr in vec![Bytecode::BrTrue(0), Bytecode::BrFalse(0)] {
+        let code = vec![Bytecode::LdU32(0), instr];
+        let module = make_module(code);
+        let fun_context = get_fun_context(&module);
+        let result = type_safety::verify(&module, &fun_context, &mut DummyMeter);
+        assert_eq!(
+            result.unwrap_err().major_status(),
+            StatusCode::BR_TYPE_MISMATCH_ERROR
+        );
+    }
+}
+*)
+Definition test_br_true_false_wrong_type (instr : file_format.Bytecode.t) : M! unit :=
+  let code := [file_format.Bytecode.LdU32 0; instr] in
+  let module := make_module code in
+  let! fun_context := get_fun_context module in
+  let! result := type_safety.verify module fun_context in
+  match result with
+  | Result.Err error =>
+    let status := error.(errors.PartialVMError.major_status) in
+    match status with
+    | errors.StatusCode.BR_TYPE_MISMATCH_ERROR => return! tt
+    | _ => panic! "unexpected status"
+    end
+  | _ => panic! "unexpected result"
+  end.
+
+Goal List.Forall
+  (fun instr => test_br_true_false_wrong_type instr = return! tt)
+  [
+    file_format.Bytecode.BrTrue 0;
+    file_format.Bytecode.BrFalse 0
+  ].
+Proof.
+  repeat constructor.
+Qed.
+
+(*
+#[test]
+#[should_panic]
+fn test_br_true_false_no_arg() {
+    for instr in vec![Bytecode::BrTrue(0), Bytecode::BrFalse(0)] {
+        let code = vec![instr];
+        let module = make_module(code);
+        let fun_context = get_fun_context(&module);
+        let _result = type_safety::verify(&module, &fun_context, &mut DummyMeter);
+    }
+}
+*)
+Definition test_br_true_false_no_arg (instr : file_format.Bytecode.t) : M!? _ unit :=
+  let code := [instr] in
+  let module := make_module code in
+  let! fun_context := get_fun_context module in
+  type_safety.verify module fun_context.
+
+Goal List.Forall
+  (fun instr =>
+    exists (Error : Set) (error : Error),
+    test_br_true_false_no_arg instr = panic! error
+  )
+  [
+    file_format.Bytecode.BrTrue 0;
+    file_format.Bytecode.BrFalse 0
+  ].
+Proof.
+  repeat econstructor.
 Qed.
